external/Goose/github_com/mit_pdos/gokv/simplepb/e.v
@@ -18,6 +18,8 @@ Definition Timeout : expr := #3.
 
 Definition EmptyConfig : expr := #4.
 
+Definition NotLeader : expr := #5.
+
 Definition EncodeError: val :=
   rec: "EncodeError" "err" :=
     marshal.WriteInt (NewSliceWithCap byteT #0 #8) "err".
